HockiKlockiLean/HockiKlockiLean/Constraints.lean
@@ -1,25 +1,46 @@
 import HockiKlockiLean.Model
+import HockiKlockiLean.Inclusion
 
 structure FilteredDimSetVar where
   dim_set_var : DimSetVar
   filtered : Set Dim
 
+def In := Dim → DimSetVar → Prop
+
 def NotIn := Dim → DimSetVar → Prop
 
 def InUnion := Dim → Set DimSetVar → Prop
 
-def InducedBy := DimSetVar → Set FilteredDimSetVar → Prop
+inductive NotInGen (rel : NotIn) : NotIn
+| given {a X} : rel a X → NotInGen rel a X
+| induced {a X Z} {R : DimSetVarRel a} : rel a X → R Z X → NotInGen rel a Z
 
-def NotIn_wf (notIn : NotIn) (f : DimSetAssignment)
-    := ∀ {a X}, notIn a X → a ∉ f X
+inductive InGen (rel : In) : In
+| given {a X} : rel a X → InGen rel a X
+| induced {a X Y} {R : DimSetVarRel a} : rel a X → R X Y → InGen rel a X
 
-def InUnion_wf (inUnion : InUnion) (f : DimSetAssignment)
-    := ∀ {a Xs}, inUnion a Xs → a ∈ (⋃ X ∈ Xs, f X)
+inductive InUnionGen (rel : InUnion) : InUnion
+| given {a Xs} : rel a Xs → InUnionGen rel a Xs
+| induced {a Xs} {R : DimSetVarRel a} : rel a Xs → InUnionGen rel a {Z | ∃ X ∈ Xs, R Z X}
 
-def InducedBy_wf (inducedBy : InducedBy) (f : DimSetAssignment)
-    := ∀ {induced inducers},
-      inducedBy induced inducers
-      →
-      ∀ inducer ∈ inducers,
-      ∀ a, a ∉ inducer.filtered
-      → a ∈ f inducer.dim_set_var → a ∈ f induced
+def In_wf (rel : In) (f : DimSetAssignment) :=
+  ∀ {a X}, rel a X → a ∈ f X
+
+def NotIn_wf (rel : NotIn) (f : DimSetAssignment) :=
+  ∀ {a X}, rel a X → a ∉ f X
+
+def InUnion_wf (rel : InUnion) (f : DimSetAssignment) :=
+  ∀ {a Xs}, rel a Xs → a ∈ (⋃ X ∈ Xs, f X)
+
+structure SchemaTy where
+  ins : Set In
+  notIns : Set NotIn
+  inUnions : Set InUnion
+  relations : (a : Dim) → DimSetVarRel a
+
+def assignment_wf (ty : SchemaTy) (f : DimSetAssignment) :=
+  ∀ c ∈ ty.ins, In_wf c f
+  → ∀ c ∈ ty.notIns, NotIn_wf c f
+  → ∀ c ∈ ty.inUnions, InUnion_wf c f
+  → ∀ a, R_wf (ty.relations a) f
+  → Prop
